src/3d/GeneralizeProbes.fst
@@ -1,0 +1,250 @@
+(*
+   Copyright 2025 Microsoft Research
+
+   Licensed under the Apache License, Version 2.0 (the "License");
+   you may not use this file except in compliance with the License.
+   You may obtain as copy of the License at
+
+       http://www.apache.org/licenses/LICENSE-2.0
+
+   Unless required by applicable law or agreed to in writing, software
+   distributed under the License is distributed on an "AS IS" BASIS,
+   WITHOUT WARRANTIES OR CONDITIONS OF ANY KIND, either express or implied.
+   See the License for the specific language governing permissions and
+   limitations under the License.
+*)
+module GeneralizeProbes
+(*
+  This module implements a pass over the source AST, run after the name resolution pass
+  of Desugar.
+
+  It generalizes types that contain probes, allowing those probes to be
+  instantiated in different ways, preparing for a subsequent specialization of
+  probed types to 32- or 64-bit layouts
+
+*)
+open FStar.Mul
+open FStar.List.Tot
+open Ast
+open FStar.All
+module H = Hashtable
+module B = Binding
+open GlobalEnv
+
+type env = Binding.env & list ident'
+let simple_probe_name_for_type (e:env) (type_name:ident)
+: option ident
+= if List.mem type_name.v (snd e)
+  then (
+    let name = reserved_prefix ^ "probe_" ^ type_name.v.name in
+    let id = { type_name with v = { type_name.v with name } } in
+    Some id
+  )
+  else None
+let mark_for_probe (e:env) (id:ident) : ML env = fst e, id.v :: snd e
+let rec head_type (e:env) (t:typ) : ML ident =
+  match (Binding.unfold_typ_abbrev_only (fst e) t).v with
+  | Type_app hd _ _ _ -> hd
+  | Pointer t _ -> head_type e t
+  | _ -> failwith 
+          (Printf.sprintf "head_type: not a type application; got %s" (print_typ t))
+
+let atomic_field_has_simple_probe (e:env) (f:atomic_field)
+: bool
+= match f.v.field_probe with
+  | Some { probe_block = { v = Probe_action_simple _ l } } -> (
+    match l.v with
+    | App SizeOf [_] -> true
+    | _ -> false
+  )
+  | _ -> false
+
+let rec needs_probe_field (e:env) (f:field)
+: ML env
+= match f.v with
+  | AtomicField f -> 
+    if atomic_field_has_simple_probe e f
+    then mark_for_probe e (head_type e f.v.field_type)
+    else e
+  | RecordField r _ -> List.fold_left needs_probe_field e r
+  | SwitchCaseField sw _ -> List.fold_left needs_probe_case e (snd sw)
+
+and needs_probe_case (e:env) (c:case)
+: ML env
+= match c with
+  | Case _ f -> needs_probe_field e f
+  | DefaultCase f -> needs_probe_field e f
+
+let need_probe_decl (e:env) (d:decl) 
+: ML env
+= match d.d_decl.v with
+  | Record _ _ _ _ fields -> List.fold_left needs_probe_field e fields
+  | CaseType _ _ _ sw -> List.fold_left needs_probe_case e (snd sw)
+  | _ -> e
+
+let need_probe_decls (e:env) (ds:list decl) = List.fold_left need_probe_decl e ds
+
+let should_generalize (e:env) (n:typedef_names) = List.mem n.typedef_abbrev.v (snd e)
+
+let generate_probe_functions (e:env) (d:decl)
+: ML (list decl)
+= match d.d_decl.v with
+  | Record names gs params w fields -> (
+    if not <| should_generalize e names
+    then [d]
+    else (
+      let Some simple_probe_name = simple_probe_name_for_type e names.typedef_abbrev in 
+      let probe_size =
+        with_range (
+          App SizeOf [with_range (Identifier names.typedef_abbrev) names.typedef_name.range]
+        ) d.d_decl.range
+      in
+      let simple_probe =
+        with_range (
+          Probe_action_simple None probe_size
+        ) d.d_decl.range
+      in
+      let d' = 
+        mk_decl 
+          (ProbeFunction simple_probe_name [] simple_probe)
+          dummy_range
+          []
+          false
+      in
+      [d;d']
+    )
+  )
+  | CaseType names gs params sw -> (
+    if not <| should_generalize e names
+    then failwith "Cannot automatically generate a probe function for a case type"
+    else (
+      [d]
+    )
+  )
+  | _ -> [d]
+
+let generalized_record_name (e:env) (n:typedef_names)
+: ML typedef_names
+= let name = reserved_prefix ^ "generalized_" ^ n.typedef_name.v.name in
+  let name = { n.typedef_name with v = { n.typedef_name.v with name } } in
+  let abbrev = reserved_prefix ^ "generalized_" ^ n.typedef_abbrev.v.name in
+  let abbrev = { n.typedef_abbrev with v = { n.typedef_abbrev.v with name = abbrev } } in
+  { typedef_name = name;
+    typedef_abbrev = abbrev;
+    typedef_ptr_abbrev = None;
+    typedef_attributes = List.filter Aligned? n.typedef_attributes }
+
+let rec generalize_probe_field (e:env) (path_prefix:string) (f:field) 
+: ML (field & list generic_param & list generic_inst)
+= match f.v with
+  | AtomicField af -> (
+    if not <| atomic_field_has_simple_probe e af
+    then f, [], []
+    else (
+      let Some probe_call = af.v.field_probe in
+      let generic_name = 
+        with_range (
+          to_ident' <|
+          reserved_prefix ^ "probe_" ^ path_prefix ^ print_ident af.v.field_ident
+        ) f.range
+      in
+      let probe = with_range (Probe_action_var generic_name) f.range in
+      let head_type = head_type e af.v.field_type in
+      match simple_probe_name_for_type e head_type with
+      | None -> f, [], []
+      | Some probe_inst ->
+        let probe_inst = with_range (Identifier probe_inst) f.range in
+        let probe_call = { probe_call with probe_block = probe } in
+        let af = { af with v = { af.v with field_probe = Some probe_call } } in
+        let f = { f with v = AtomicField af } in
+        f, [GenericProbeFunction generic_name], [ probe_inst]
+    )
+  )
+  | RecordField r i ->
+    let path_prefix = path_prefix ^ print_ident i in
+    let r, gs, insts = generalize_probe_fields e path_prefix r in
+    { f with v = RecordField r i }, gs, insts
+  | SwitchCaseField sw i ->
+    let path_prefix = path_prefix ^ print_ident i in
+    let cs, gs, insts = generalize_probe_cases e path_prefix (snd sw) in
+    { f with v = SwitchCaseField (fst sw, cs) i }, gs, insts
+  
+and generalize_probe_case (e:env) (path_prefix:string) (c:case)
+: ML (case & list generic_param & list generic_inst)
+= match c with
+  | Case ex f ->
+    let f, gs, insts = generalize_probe_field e path_prefix f in
+    Case ex f, gs, insts
+  | DefaultCase f ->
+    let f, gs, insts = generalize_probe_field e path_prefix f in
+    DefaultCase f, gs, insts
+
+and generalize_probe_fields (e:env) (path_prefix:string) (fs:list field) 
+: ML (list field & list generic_param & list generic_inst)
+= List.fold_right 
+    (fun f (fs, gs, is) -> 
+       let f, gs', is' = generalize_probe_field e path_prefix f in
+       f::fs, gs'@gs, is'@is)
+    fs ([], [], [])
+
+and generalize_probe_cases (e:env) (path_prefix:string) (cs:list case)
+: ML (list case & list generic_param & list generic_inst)
+= List.fold_right 
+    (fun f (fs, gs, is) -> 
+       let f, gs', is' = generalize_probe_case e path_prefix f in
+       f::fs, gs'@gs, is'@is)
+    cs ([], [], [])
+
+let generalize_probes_decl (e:env) (d:decl)
+: ML (list decl)
+= match d.d_decl.v with
+  | Record names gs params w fields -> (
+    let fields, gs', insts = generalize_probe_fields e "" fields in
+    match gs' with
+    | [] -> [d]
+    | _ -> (
+      let gen_name = generalized_record_name e names in
+      let generalized_record =
+        { d with 
+          d_decl = { d.d_decl with 
+          v=Record gen_name (gs'@gs) params w fields }}
+      in
+      let instantiated_type =
+        let head = gen_name.typedef_abbrev in
+        let instantiations =
+          insts @
+          List.map
+            (function GenericProbeFunction i ->
+              with_range (Identifier i) i.range)
+            gs
+        in
+        let params =
+          List.map (fun (_, i, _) -> Inl <| with_range (Identifier i) i.range) params
+        in
+        with_range (Type_app head KindSpec instantiations params)
+                    d.d_decl.range
+      in
+      let inst_attrs = List.filter (fun a -> not (Aligned? a)) names.typedef_attributes in
+      let instantiated_record =
+        { d with 
+          d_decl = { d.d_decl with 
+          v=TypeAbbrev inst_attrs instantiated_type names.typedef_abbrev gs params }}
+      in
+      [generalized_record; instantiated_record]
+    )
+  )
+  | CaseType _ _ _ _ -> generate_probe_functions e d
+  | _ -> [d]
+
+let generalize_probe_decls (e:GlobalEnv.global_env) (ds:list decl)
+: ML (list decl)
+= let e = Binding.mk_env e, [] in
+  let e = need_probe_decls e ds in
+  let print_ident (i:ident') = i.name in
+  FStar.IO.print_string 
+    (Printf.sprintf "Probes needed for: %s\n" 
+      (String.concat ", " (List.map print_ident (snd e))));
+  let ds = List.collect (generate_probe_functions e) ds in
+  FStar.IO.print_string
+    (Printf.sprintf "Generated probe functions\n%s\n" (print_decls ds));
+  List.collect (generalize_probes_decl e) ds
