src/3d/Main.fst
@@ -64,6 +64,12 @@ let parse_check_and_desugar (en:env) (mname:string) (fn:string)
   Options.debug_print_string (print_decls decls);
   Options.debug_print_string "\n";
 
+  let decls = GeneralizeProbes.generalize_probe_decls en.binding_env decls in
+
+  Options.debug_print_string "=============After probe generalization=============\n";
+  Options.debug_print_string (print_decls decls);
+  Options.debug_print_string "\n";
+
   let decls, benv = Binding.bind_decls en.binding_env decls in
 
   Options.debug_print_string "=============After binding=============\n";
